KripkeGameAnalysis/Generic/SetoidWithCanonicalizer.lean
@@ -1,0 +1,16 @@
+class SetoidWithCanonicalizer (α : Type) extends Setoid α where
+  canonicalize : α → α
+  canonicalize_equiv_self : ∀ x, canonicalize x ≈ x
+  equiv_then_canonicalize_eq : ∀ x y, x ≈ y → canonicalize x = canonicalize y
+
+namespace SetoidWithCanonicalizer
+
+theorem canonicalize_eq_iff_equiv [SetoidWithCanonicalizer α] (f f' : α) : canonicalize f = canonicalize f' ↔ f ≈ f' := by
+  apply Iff.intro
+  · intro h
+    have p1 : f ≈ canonicalize f := Setoid.iseqv.symm (canonicalize_equiv_self f)
+    rw [h] at p1
+    exact (Setoid.iseqv.trans p1 (canonicalize_equiv_self f'))
+  · exact SetoidWithCanonicalizer.equiv_then_canonicalize_eq f f'
+
+end SetoidWithCanonicalizer
